src/program_proof/simplefs/inode_proof.v
@@ -12,6 +12,7 @@ From RecordUpdate Require Import RecordSet.
 Import RecordSetNotations.
 
 Set Default Proof Using "Type".
+#[local] Unset Printing Projections.
 
 Module inodeType.
 Inductive t :=
@@ -100,7 +101,7 @@ Definition is_meta (v: val) (meta: w32) :=
 
 Theorem wp_Meta__AsBytes (meta: w32) :
   {{{ True }}}
-    Meta__AsBytes (#meta, #())
+    Meta__AsBytes (#meta, #())%V
   {{{ (s : Slice.t), RET (to_val s); own_slice s byteT (DfracOwn 1) (u32_le meta) }}}.
 Proof.
   (*@ func (m *Meta) AsBytes() []byte {                                       @*)
@@ -204,5 +205,183 @@ Proof.
   wp_rec. wp_storeField. iModIntro. iApply "HΦ".
   iFrame.
 Qed.
+
+Theorem wp_Inode__AsBytes (i : loc) ino :
+  {{{ own_inode i ino }}}
+    Inode__AsBytes #i
+  {{{ (s : Slice.t), RET (to_val s); own_slice s byteT (DfracOwn 1) (inode_rep.encode ino) ∗
+                                     own_inode i ino }}}.
+Proof.
+  (*@ func (i *Inode) AsBytes() []byte {                                      @*)
+  (*@     var buf = make([]byte, 0)                                           @*)
+  (*@     buf = marshal.WriteInt32(buf, uint32(i.typ_))                       @*)
+  (*@     buf = marshal.WriteInt(buf, i.length)                               @*)
+  (*@     buf = append(buf, i.meta.AsBytes()...)                              @*)
+  (*@     for _, ptr := range i.blockPtrs {                                   @*)
+  (*@         buf = marshal.WriteInt32(buf, ptr)                              @*)
+  (*@     }                                                                   @*)
+  (*@     return buf                                                          @*)
+  (*@ }                                                                       @*)
+  iIntros (Φ) "Hpre HΦ". iDestruct "Hpre" as "Hi". iNamed "Hi".
+  wp_rec. wp_pures.
+  wp_apply (wp_NewSlice_0). iIntros (s1) "Hs".
+  wp_apply wp_ref_to; [ auto | ]. iIntros (buf_l) "buf".
+  wp_pures.
+  wp_loadField. wp_load.
+  wp_apply (wp_WriteInt32 with "[$]").
+  iIntros (s2) "Hs".
+  wp_store. wp_loadField. wp_load.
+  wp_apply (wp_WriteInt with "[$]").
+  iIntros (s3) "Hs".
+  wp_store. wp_loadField. wp_apply wp_Meta__AsBytes.
+  iIntros (meta_s) "Hs_meta".
+  iApply own_slice_to_small in "Hs_meta".
+  wp_load. wp_apply (wp_SliceAppendSlice with "[$Hs $Hs_meta]"); first done.
+  iIntros (s4) "[Hs _]".
+  rewrite app_nil_l.
+  wp_store.
+  wp_loadField.
+
+  set (ino_bs0 := (u32_le (inodeType.rep ino.(inode_rep.typ)) ++ u64_le ino.(inode_rep.len)) ++
+    u32_le ino.(inode_rep.meta)).
+
+  iDestruct (own_slice_small_sz with "HblockPtrs") as %Hs_sz.
+  assert (uint.Z s.(Slice.sz) = 28).
+  { move: Hs_sz. len. }
+
+  wp_apply
+    (wp_forSlice (λ (i: w64),
+         ∃ (s': Slice.t),
+           "buf" ∷ buf_l ↦[slice.T byteT] s' ∗
+           "Hs" ∷ own_slice s' byteT (DfracOwn 1)
+             (ino_bs0 ++
+                concat (u32_le <$> (take (uint.nat i) ino.(inode_rep.block_ptrs)))))%I
+                 with "[] [$HblockPtrs $buf Hs]"
+    ).
+  { iIntros (n x).
+    clear Φ.
+    iIntros "!>" (Φ) "(I & %Hn & %Hget) HΦ".
+    iNamed "I".
+    wp_pures. wp_load.
+    wp_apply (wp_WriteInt32 with "[$Hs]").
+    iIntros (s'') "Hs".
+    wp_store.
+    iModIntro.
+    iApply "HΦ".
+    iFrame.
+    iExactEq "Hs".
+    rewrite /named.
+    f_equal.
+    rewrite -app_assoc.
+    f_equal.
+    replace (uint.nat (word.add n (W64 1))) with (S (uint.nat n)) by word.
+    erewrite take_S_r; eauto.
+    rewrite fmap_app /= concat_app //.
+  }
+  { iExactEq "Hs". rewrite /named.
+    rewrite take_0. rewrite fmap_nil concat_nil app_nil_r //. }
+  iIntros "(I & HblockPtrs)". iNamed "I".
+  wp_load. iModIntro. iApply "HΦ". iFrame.
+  iExactEq "Hs".
+  f_equal.
+  rewrite take_ge; [ | len ].
+  rewrite /inode_rep.encode //.
+Qed.
+
+Opaque concat.
+
+Theorem wp_FromBytes (b : Slice.t) bs ino :
+  {{{ own_slice b byteT (DfracOwn 1) bs ∗ ⌜bs = inode_rep.encode ino⌝ }}}
+    FromBytes (to_val b)
+  {{{ (l : loc), RET #l; own_inode l ino }}}.
+Proof.
+  (*@ func FromBytes(b []byte) *Inode {                                       @*)
+  (*@     typ, b2 := marshal.ReadInt32(b)                                     @*)
+  (*@     length, b3 := marshal.ReadInt(b2)                                   @*)
+  (*@     meta, b4 := metaFromBytes(b3)                                       @*)
+  (*@     blockPtrs := make([]uint32, NUM_BLOCK_PTRS)                         @*)
+  (*@     var bytes = b4                                                      @*)
+  (*@     for idx := range blockPtrs {                                        @*)
+  (*@         ptr, b_next := marshal.ReadInt32(bytes)                         @*)
+  (*@         bytes = b_next                                                  @*)
+  (*@         blockPtrs[idx] = ptr                                            @*)
+  (*@     }                                                                   @*)
+  (*@     return &Inode{                                                      @*)
+  (*@         typ_:      simplefs.InodeType(typ),                             @*)
+  (*@         length:    length,                                              @*)
+  (*@         meta:      meta,                                                @*)
+  (*@         blockPtrs: blockPtrs,                                           @*)
+  (*@     }                                                                   @*)
+  (*@ }                                                                       @*)
+  iIntros (Φ) "Hpre HΦ". iDestruct "Hpre" as "[Hbs %]". subst.
+  wp_rec. wp_pures.
+  iApply own_slice_to_small in "Hbs".
+  wp_apply (wp_ReadInt32 with "[$]").
+  iIntros (s1) "Hs". wp_pures.
+  wp_apply (wp_ReadInt with "[$]").
+  iIntros (s2) "Hs". wp_pures.
+  wp_apply (wp_metaFromBytes with "[$Hs]").
+  iIntros (s3) "Hs". wp_pures.
+  wp_apply (wp_NewSliceWithCap_0). iIntros (bptrs_s) "[Hblkptrs _]".
+  wp_apply wp_ref_to; [ done | ]. iIntros (l) "blockPtrs".
+  wp_apply wp_ref_to; [ done | ]. iIntros (l2) "bytes".
+  wp_apply wp_ref_to; [ auto | ]. iIntros (l3) "i".
+  wp_pures.
+  change (word.add (W64 27) (W64 1)) with (W64 28).
+  wp_apply (wp_forUpto
+              (λ (i: w64),
+                ∃ (bptrs_s: Slice.t) (s': Slice.t),
+                "bytes" ∷ l2 ↦[slice.T byteT] s' ∗
+                "Hs" ∷ own_slice_small s' byteT (DfracOwn 1)
+                       (concat (u32_le <$> (drop (uint.nat i) (ino.(inode_rep.block_ptrs))))) ∗
+                "blockptrs" ∷ l ↦[slice.T uint32T] bptrs_s ∗
+                "Hblkptrs" ∷ own_slice bptrs_s uint32T (DfracOwn 1)
+                  (take (uint.nat i) (ino.(inode_rep.block_ptrs)))
+              )%I with "[] [$bytes $blockPtrs Hblkptrs Hs $i] "
+           ).
+  { word. }
+  { iIntros (i). clear Φ.
+    iIntros "!>" (Φ) "(I & i & %Hi) HΦ". iNamed "I".
+    wp_pures.
+    wp_load.
+    assert (∃ ptr, vec_to_list ino.(inode_rep.block_ptrs) !! uint.nat i = Some ptr)
+      as [ptr Hgeti].
+    { apply lookup_lt_is_Some_2. len. }
+    wp_apply (wp_ReadInt32 with "[Hs]").
+    { erewrite drop_S; [ | eauto ].
+      rewrite fmap_cons concat_cons. eauto. }
+    iIntros (s'') "Hs".
+    wp_pures. wp_store. wp_load.
+    change (#ptr) with (to_val ptr).
+    wp_apply (wp_SliceAppend with "[$Hblkptrs]").
+    iIntros (bptrs_s') "Hblkptrs".
+    wp_store.
+    iModIntro. iApply "HΦ".
+    iFrame.
+    rewrite /named.
+    iSplitL "Hs".
+    - iExactEq "Hs".
+      repeat (f_equal; try word).
+    - iExactEq "Hblkptrs".
+      f_equal.
+      replace (uint.nat (word.add i (W64 1))) with (S (uint.nat i)) by word.
+      erewrite take_S_r; eauto.
+  }
+  {
+    (* initial invariant *)
+    rewrite drop_0 take_0. iFrame.
+  }
+  iIntros "(I & _)". iNamed "I".
+  wp_load.
+  wp_apply wp_allocStruct; [ val_ty | ].
+  iIntros (l4) "Hino".
+  iApply struct_fields_split in "Hino". iNamed "Hino".
+  iApply "HΦ".
+  iFrame.
+  iApply own_slice_to_small in "Hblkptrs".
+  rewrite take_ge; [ | len ].
+  iFrame.
+Qed.
+
 
 End proof.
